seq-embed/test_deriv.lean
@@ -1,0 +1,5 @@
+import NfValidate
+import SeqEmbed.Basic
+
+def phi1 : Formula := Formula.eq (Var.bound 0) (Var.free "z")
+#eval checkStrat phi1
